Confidential send and receive function and example protocol

examples/single_message/DY.Example.SingleMessage.SecurityProperties.fst
@@ -7,35 +7,19 @@ open DY.Example.SingleMessage.Protocol.Total.Proof
 open DY.Example.SingleMessage.Protocol.Stateful
 open DY.Example.SingleMessage.Protocol.Stateful.Proof
 
-#set-options "--fuel 0 --ifuel 1 --z3rlimit 25  --z3cliopt 'smt.qi.eager_threshold=100'"
+#set-options "--fuel 0 --ifuel 0 --z3rlimit 10  --z3cliopt 'smt.qi.eager_threshold=100'"
 
-val receiver_authentication:
-  tr:trace -> i:timestamp ->
-  sender:principal -> receiver:principal -> secret:bytes ->
-  Lemma
-  (requires
-    trace_invariant tr /\
-    event_triggered_at tr i sender (ClientSendMsg sender receiver secret)
-  )
-  (ensures
-    is_corrupt tr (principal_label sender) \/ is_corrupt tr (principal_label receiver) \/
-    (exists i'. event_triggered i' receiver (ServerReceivedMsg sender receiver secret))
-  )
-let receiver_authentication tr i sender receiver secret = admit()
-
-val secret_secrecy:
+val secret_secrecy_sender:
   tr:trace -> sender:principal -> receiver:principal -> secret:bytes ->
   Lemma
   (requires
     trace_invariant tr /\
     attacker_knows tr secret /\
-    ((exists sess_id. state_was_set tr sender sess_id (ClientState receiver secret)) \/
-    (exists sess_id. state_was_set tr receiver sess_id (ServerState secret)))
+    (exists sess_id. state_was_set tr sender sess_id (ClientState receiver secret))
   )
   (ensures
     is_corrupt tr (principal_label sender) \/ is_corrupt tr (principal_label receiver)
   )
-let secret_secrecy tr sender receiver secret =
+let secret_secrecy_sender tr sender receiver secret =
   attacker_only_knows_publishable_values tr secret;
-  admit();
   ()
