src/lib/communication/DY.Lib.Communication.API.Predicates.fst
@@ -1,0 +1,51 @@
+module DY.Lib.Communication.API.Predicates
+
+open Comparse
+open DY.Core
+open DY.Lib.Crypto.PkEncryption.Split
+open DY.Lib.Event.Typed
+
+open DY.Lib.Communication.API
+
+#set-options "--fuel 0 --ifuel 0 --z3cliopt 'smt.qi.eager_threshold=100'"
+
+(*** Cryptographic Predicates ***)
+
+// TODO add higher layer preds as a parameter
+#push-options "--ifuel 2 --fuel 0"
+val pkenc_crypto_predicates_communication_layer: cusages:crypto_usages -> pkenc_crypto_predicate cusages
+let pkenc_crypto_predicates_communication_layer cusages = {
+  pred = (fun tr pk msg ->
+    get_sk_usage pk == PkKey comm_layer_tag empty /\
+      (match parse communication_message msg with
+      | Some {sender; receiver; payload} -> (
+        get_sk_label pk == principal_label receiver /\
+        (get_label payload) `can_flow tr` (join (principal_label sender) (principal_label receiver))
+      )
+      | None -> False)
+    );
+  pred_later = (fun tr1 tr2 pk msg -> ());
+}
+#pop-options
+
+val pkenc_crypto_predicates_communication_layer_and_tag: 
+  {|cusages:crypto_usages|} ->
+  (string & pkenc_crypto_predicate cusages)
+let pkenc_crypto_predicates_communication_layer_and_tag #cusages = 
+  (comm_layer_tag, pkenc_crypto_predicates_communication_layer cusages)
+
+val has_communication_layer_invariants:
+  crypto_invariants ->
+  prop
+let has_communication_layer_invariants cinvs =
+  has_pkenc_predicate cinvs pkenc_crypto_predicates_communication_layer_and_tag
+
+(*** Event Predicates ***)
+
+#push-options "--ifuel 1 --fuel 0"
+let event_predicate_communication_layer {|cinvs:crypto_invariants|} : event_predicate communication_event =
+  fun tr prin e ->
+    match e with
+    | CommunicationLayerSendMsg sender receiver payload -> True
+    | CommunicationLayerReceiveMsg sender receiver payload -> True
+#pop-options
